**Question 1:**

$$ L = \frac{1}{2}[-A\dot{t}^2 + B\dot{r}^2 + r^2 \dot{θ}^2 + r^2sin^2(θ)\dot{ϕ}^2]$$

$$ P_\phi = \frac{\partial L}{\partial \dot{\phi}} = r^2sin^2(\theta)\dot{\phi} $$

$$ P_t = \frac{\partial L}{\partial \dot{t}} = -A \dot{t}  $$

$$ P_r = \frac{\partial L}{\partial \dot{r}} = B\dot{r} $$

$$ P_θ = \frac{\partial L}{\partial \dot{\theta}} = 0 $$

Since $\theta$ given as a constant, $ \theta = \space\frac{π}{2} $, from Euler-Lagrange equation $ P_\theta = 0 .$ Where $L_z = P_\phi $ and $ -E= P_t $ we can write   $ \dot{\phi} = \frac{L_z}{r^2}$, $ \dot{t} = \frac{E}{A}, $  $ \dot{r} = \frac{P_r}{B} $. 

Also $ \dot{x}^\alpha = P^\alpha $ and $ g^{rr} = \frac{1}{B} $ are given in the article. So we can say that,
$$ \dot{x}^r = g^{rr} {P_r} = \frac{1}{B} {P_r} =  \dot{r}. $$

Plugging these values with $ \dot{r} = \frac{dr}{dλ}$ into our Lagrangian, which we take 0 for a photon, we find the following result:

$$ 0 = -\frac{1}{A} E^2 + \frac{1}{B} \bigg(\frac{dr}{dλ} \bigg)^2 + \frac{1}{r^3}L_z^2 $$

**Question 2:**

* In order to find $ \frac{\partial{P_r}}{\partial{λ}} $ we can take derivative of the Lagrangian with respect to r. From Euler-Lagrange equation:

$$ \frac{\partial{L}}{\partial{r}} = \frac{\partial{}}{\partial{λ}} \bigg(\frac{\partial{L}}{\partial{\dot{r}}}\bigg) = \frac{\partial{P_r}}{\partial{λ}} $$

and

$$ \frac{\partial{L}}{\partial{r}} = \frac{1}{2} \bigg[-\frac{d}{dr} \bigg(\frac{1}{A} \bigg) + \frac{d}{dr} \bigg(\frac{1}{B} \bigg) P_r^2 -\frac{2}{r^3} L_z^2 \bigg] = \frac{\partial{P_r}}{\partial{λ}} . $$


* To find $ \frac{dr}{dλ} $ from Lagrangian:
$$ P_r = \frac{\partial{L}}{\partial{\dot{r}}} = B\dot{r} = B \frac{dr}{dλ}$$

so

$$ \frac{dr}{dλ} = \frac{P_r}{B}. $$

**Question 3:**

$$ H = \frac{1}{2}[-e^{2Φ} P_t^2 \frac{P_u^{2} + P_v^{2}}{ a^{2} \left(\sin^{2}{\left(v \right)} + \sinh^{2}{\left(u \right)}\right)} + P_z^2] $$

Our task is the showing fallowing identity is an integral of motion.

$$ P_{const} = \frac{P_u \sin{\left(v \right)} \cos{\left(v \right)} + P_v \sinh{\left(u \right)} \cosh{\left(u \right)}}{\sin^{2}{\left(v \right)} + \sinh^{2}{\left(u \right)}} $$ 

To prove this identity is an integral of motion, we must calculate the Poisson Bracket of $ p_{const} $ and $ {H} $ and show that is equals to zero i.e We must show $$ \{H, P\} = 0 $$

 $$ ∑ \frac{\partial P_{const}}{\partial q_i}  \frac{\partial H}{\partial P_i} - \frac{\partial H}{\partial q_i}  \frac{\partial P_{const}}{\partial P_i} $$ 

One can see that there is no $ z, t, P_t $ and $ P_z $ dependence on $ P_{const} $. Therefore, it is enough to calculate only $ u $ and $ v $ dependence to find the result of the Poisson Bracket.

$ u $ dependence can be calculated as $$ \frac{\partial P_{const}}{\partial u}  \frac{\partial H}{\partial P_u} - \frac{\partial H}{\partial u}  \frac{\partial P_{const}}{\partial P_u}$$ 

and the result is

$$ \frac{P_u\left(\frac{P_v \sinh^{2}{\left(u \right)} + P_v \cosh^{2}{\left(u \right)}}{\sin^{2}{\left(v \right)} + \sinh^{2}{\left(u \right)}} - \frac{2 \left(P_u\sin{\left(v \right)} \cos{\left(v \right)} + P_v \sinh{\left(u \right)} \cosh{\left(u \right)}\right) \sinh{\left(u \right)} \cosh{\left(u \right)}}{\left(\sin^{2}{\left(v \right)} + \sinh^{2}{\left(u \right)}\right)^{2}}\right)}{a^{2} \left(\sin^{2}{\left(v \right)} + \sinh^{2}{\left(u \right)}\right)} + \frac{\left(P_u^{2} + P_v^{2}\right) \sin{\left(v \right)} \cos{\left(v \right)} \sinh{\left(u \right)} \cosh{\left(u \right)}}{a^{2} \left(\sin^{2}{\left(v \right)} + \sinh^{2}{\left(u \right)}\right)^{3}} $$

After the simplifications

$$ - \frac{2 P_u \left(P_u \sin{\left(2 v \right)} \sinh{\left(2 u \right)} - 2 P_v \sin^{2}{\left(v \right)} \cosh{\left(2 u \right)} + P_v \cosh{\left(2 u \right)} - P_v\right) - \left(P_u^{2} + P_v^{2}\right) \sin{\left(2 v \right)} \sinh{\left(2 u \right)}}{4 a^{2} \left(\sin^{2}{\left(v \right)} + \sinh^{2}{\left(u \right)}\right)^{3}} $$

Same calculation fo $ v $ depencence
$$ \frac{\partial P_{const}}{\partial v}  \frac{\partial H}{\partial P_v} - \frac{\partial H}{\partial v}  \frac{\partial P_{const}}{\partial P_v}$$ 

and result is 

$$ \frac{P_v \left(\frac{- P_u \sin^{2}{\left(v \right)} + P_u \cos^{2}{\left(v \right)}}{\sin^{2}{\left(v \right)} + \sinh^{2}{\left(u \right)}} - \frac{2 \left(P_u \sin{\left(v \right)} \cos{\left(v \right)} + P_v \sinh{\left(u \right)} \cosh{\left(u \right)}\right) \sin{\left(v \right)} \cos{\left(v \right)}}{\left(\sin^{2}{\left(v \right)} + \sinh^{2}{\left(u \right)}\right)^{2}}\right)}{a^{2} \left(\sin^{2}{\left(v \right)} + \sinh^{2}{\left(u \right)}\right)} + \frac{\left(P_u^{2} + P_v^{2}\right) \sin{\left(v \right)} \cos{\left(v \right)} \sinh{\left(u \right)} \cosh{\left(u \right)}}{a^{2} \left(\sin^{2}{\left(v \right)} + \sinh^{2}{\left(u \right)}\right)^{3}} $$ 

After the simplifications

$$ - \frac{\frac{P_v \left(- P_u \cos{\left(2 v \right)} \cosh{\left(2 u \right)} + P_u + P_v \sin{\left(2 v \right)} \sinh{\left(2 u \right)}\right)}{2} - \frac{\left(P_u^{2} + P_v^{2}\right) \sin{\left(2 v \right)} \sinh{\left(2 u \right)}}{4}}{a^{2} \left(\sin^{2}{\left(v \right)} + \sinh^{2}{\left(u \right)}\right)^{3}} $$

If we add two results, we get $$ - \frac{2 P_u \left(P_u \sin{\left(2 v \right)} \sinh{\left(2 u \right)} - 2 P_v \sin^{2}{\left(v \right)} \cosh{\left(2 u \right)} + P_v \cosh{\left(2 u \right)} - P_v\right) - \left(P_u^{2} + P_v^{2}\right) \sin{\left(2 v \right)} \sinh{\left(2 u \right)}}{4 a^{2} \left(\sin^{2}{\left(v \right)} + \sinh^{2}{\left(u \right)}\right)^{3}} - \frac{\frac{P_v \left(- P_u \cos{\left(2 v \right)} \cosh{\left(2 u \right)} + P_u + P_v \sin{\left(2 v \right)} \sinh{\left(2 u \right)}\right)}{2} - \frac{\left(P_u^{2} + P_v^{2}\right) \sin{\left(2 v \right)} \sinh{\left(2 u \right)}}{4}}{a^{2} \left(\sin^{2}{\left(v \right)} + \sinh^{2}{\left(u \right)}\right)^{3}} $$ 

After simplifications we get $ 0 $. Therefore $ P_{const} $ is equation of motion.


**Question 4:**

We have such a Lagrangian 

$$ L = \frac{1}{2}\bigg(\frac{- \dot{t}^2 -2x \dot{t} \dot{x} + \dot{x}^2}{1 + x^2} \bigg) $$

Our $P_x$ value is $\frac{\partial{L}}{\partial{\dot{x}}}$ and our $P_t$ value is $\frac{\partial{L}}{\partial{\dot{t}}}$

$$ P_x = \frac{-2x \dot{t} + 2\dot{x}}{2(1+x^2)}$$

\


$$ P_t = \frac{-2 \dot{t} - 2\dot{x}x}{2(1+x^2)}$$

We can obtain the Hamiltonian by Legendre Transformation;

$$ H (p, q) = \sum{p_i \dot{q_i} - L}$$

Thus our Hamiltonian will be

$$ H(p, q) = P_x \dot{x} + P_t \dot{t} - L$$

The $\dot{x}$ value will be equal to from $P_x$ and $P_t$ values;

$$ \dot{x} = \frac{2(1 + x^2)P_x + 2x\dot{t}}{2}$$

\

$$ \dot{x} = \frac{2(1 + x^2)P_t + 2\dot{t}}{-2x}$$

If we equate them we will obtain the fallowing;

$$ \dot{x} = P_x - xP_t$$

Similarly, the $\dot{t}$ value will be equal to both from $P_x$ and $P_t$ values;

$$ \dot{t} = \frac{-2\big(1 + x^2\big)P_x + 2\dot{x}}{2x}$$

\
$$ \dot{t} = \frac{2\big(1 + x^2 \big)P_t + 2x\dot{x}}{-2}$$

If we equate them we will obtain the fallowing;

$$ \dot{t} = -P_t - xP_t$$

And, if we use partial fraction method we can obtain that;

$$ L = \frac{1}{2} \bigg[\frac{- \dot{t}^2 -x\dot{x} \dot{t}}{1 + x^2} + \frac{-\dot{x} x t + \dot{x}^2}{1 + x^2} \bigg] $$

Which is equal to;

$$ L = \frac{1}{2}[\dot{t} P_t + \dot{x} P_x]$$

By Legendre Transformation, our Hamiltonian will be equal to;

$$ H (p, q) = \frac{1}{2} \big( \dot{x} P_x + \dot{t} P_t\big)$$

If we plug-in the values that we found above ($ \dot{x} $ and $ \dot{t} $) we will obtain that;

$$ H(p, q) = \frac{1}{2} (P_x^2 - P_t^2 - 2xP_x P_t)$$

as needed.

**Question 5:**

$$ L = \frac{1}{2} \bigg (\frac{-\dot t -2x \dot t \dot x + \dot x^2}{1 + x^2} \bigg )      $$

Euler-Lagrange equation is 

$$ \frac{\partial L}{\partial t } - \frac{dL}{dt} \bigg( \frac{\partial L}{\partial \dot t }  \bigg)  = 0 $$

Since there is no t dependence in Lagrangian we have 

$$   \frac{dL}{dt} \bigg( \frac{\partial L}{\partial \dot t }  \bigg)  = 0   $$

then we have

$$ \frac{\partial L}{\partial \dot t } = P_t = constant $$


$$ P_t = \frac{-\dot t + x \dot x}{1+ x^2} = constant $$

By using Noether's Theorem, 

$$ \frac{\partial L}{\partial \dot q } \frac{df}{d\epsilon} \bigg|_{\epsilon=0} = \textit{Integral of motion} $$
as
$$ t \rightarrow t + \epsilon \\  f(t) = t + \epsilon $$
